menagerie.v
@@ -6,7 +6,7 @@ Notation "'transp' P e x" := (eq_rect _ P x _ e)
   (at level 10, P at next level, e at next level, x at next level, no associativity).
 Scheme eq_indd := Induction for eq Sort Prop.
 Lemma eq_rect_cst (A:Type) (x y:A) (e:x=y) (P:Type) (p:P) :
-  eq_rect x (fun _ => P) p y e = p.
+  transp (fun _ => P) e p = p.
 case e; reflexivity.
 Qed.
 Definition dmap {X:Type}{Y:X->Type}(f:forall x:X,Y x){x x':X}(e:x=x')
@@ -39,6 +39,64 @@ fixmatch {h} c as c0 return (P c0) with
 end
 *)
 
+Print Circle_rect2.
+(*
+Circle_rect2 = 
+fun (P : Circle -> Type) (f : P base) (g : transp P loop f = f)
+  (c c0 : Circle) (e : c = c0) =>
+fixmatch {h} e as c1 return (P c1) with
+| base => f
+| loop _ => g
+end
+     : forall (P : Circle -> Type) (f : P base) (g : transp P loop f = f)
+         (c c0 : Circle) (e : c = c0),
+       transp (fun c1 : Circle => P c1) e
+       fixmatch {h} c as c1 return (P c1) with
+       | base => f
+       | loop _ => g
+       end =
+       fixmatch {h} c0 as c1 return (P c1) with
+       | base => f
+       | loop _ => g
+       end
+*)
+Check (Circle_rect2 : forall
+ (P:Circle->Type) (pt:P base) (lp:transp P loop pt = pt) c c' (w:c=c'),
+ transp P w (Circle_rect P pt lp c) = Circle_rect P pt lp c').
+
+Section CircleComputation.
+
+Variable P : Circle -> Type.
+Variable pt : P base.
+Variable lp : transp _ loop pt = pt.
+
+Eval compute in Circle_rect P pt lp base. (* = pt *)
+
+Lemma compute_base : Circle_rect P pt lp base = pt.
+Proof (refl_equal pt). (* definitional equality *)
+
+Lemma compute_loop :
+      dmap (Circle_rect P pt lp) loop = lp.
+(* uses: (Circle_rect2 ... loop) reduces to lp *)
+change (dmap (Circle_rect P pt lp) loop = Circle_rect2 P pt lp _ _ loop).
+case loop.
+(* uses: (Circle_rect2 ... eq_refl) reduces to eq_refl (and the usual reduction of J) *)
+lazy beta delta iota.
+reflexivity.
+Qed.
+Print compute_loop. (* propositional equality *)
+
+Eval compute in transp P loop pt.
+(* A match over a constructor, and it does not compute!
+       match loop in (_ = y) return (P y) with
+       | eq_refl => pt
+       end
+ => canonicity lost!
+*)
+
+End CircleComputation.
+
+
 Inductive Circle' : Type :=
   | east : Circle'
   | west : Circle'
@@ -56,30 +114,28 @@ Circle'_rect
 
 Require Import Program.
 
-Program Definition Circle'2Circle (c:Circle') : Circle :=
-  Circle'_rect (fun _ => Circle) base base _ _ c.
-Next Obligation.
-apply eq_rect_cst.
+Lemma C2C_ob1 : transp (fun _ : Circle' => Circle) upper base = base.
+rewrite eq_rect_cst.
+apply eq_refl.
 Defined.
-Next Obligation.
-apply eq_rect_cst.
+Lemma C2C_ob2 : transp (fun _ : Circle' => Circle) lower base = base.
+rewrite eq_rect_cst.
+apply loop.
 Defined.
+
+Definition Circle'2Circle (c:Circle') : Circle :=
+  Circle'_rect (fun _ => Circle) base base C2C_ob1 C2C_ob2 c.
 
 Program Definition Circle2Circle' (c:Circle) : Circle' :=
   Circle_rect (fun _ => Circle') east _ c.
 Next Obligation.
-apply eq_rect_cst.
+rewrite eq_rect_cst.
+transitivity west.
+ apply lower.
+ apply upper.
 Defined.
 
 Eval compute in Circle2Circle' base.
-
-Eval compute in fun (P:Circle->Type) (x:P base) =>
-  transp P loop x.
-(* A match over a constructor, and it does not compute!
-       match loop in (_ = y) return (P y) with
-       | eq_refl => x
-       end
-*)
 
 Inductive Interval : Type :=
     | left : Interval
@@ -101,7 +157,7 @@ fun (P : Interval -> Type) (f : P left) (f0 : P right)
 match i as i0 return (P i0) with
 | left => f
 | right => f0
-| segment x => g x
+| segment _ => g
 end
 *)
 
@@ -110,7 +166,6 @@ eapply Interval_rect with (i:=x).
 Show Existentials.
 instantiate (1:=eq_refl).
 instantiate (1:=segment).
-unfold eq_rect.
 exact (eq_indd _ left (fun z (e:left=z) =>
   match e in _=y return y=z with eq_refl => e end = @eq_refl _ z) eq_refl right segment).
 Defined.
@@ -139,6 +194,11 @@ Susp_rect
          (f0 : P (south X)),
        (forall x : X, transp P (merid X x) f = f0) -> forall s : Susp X, P s
 *)
+Check (Susp_rect2 :
+  forall X P (f:P(north X)) (f0:P(south X)) (g:forall x:X, transp P (merid X x) f = f0)
+    (s s' : Susp X) (e:s=s'),
+  transp P e (Susp_rect X P f f0 g s) = Susp_rect X P f f0 g s').
+
 
 Inductive Cyl {X Y : Type} (g : X -> Y) : Y -> Type :=
     | cyl_base : forall y:Y, Cyl g y
@@ -155,6 +215,13 @@ Cyl_rect
        (forall x : X, transp (P (g x)) (cyl_seg X Y g x) (f0 x) = f (g x)) ->
        forall (y : Y) (c : Cyl g y), P y c
 *)
+Check (Cyl_rect2 : forall (X Y : Type) (g : X -> Y) (P : forall y : Y, Cyl g y -> Type)
+         (f : forall y : Y, P y (cyl_base g y))
+         (f0 : forall x : X, P (g x) (cyl_top g x))
+         (g0:forall x : X, transp (P (g x)) (cyl_seg X Y g x) (f0 x) = f (g x))
+         (y : Y) (c c' : Cyl g y) (e:c=c'),
+  transp (P y) e (Cyl_rect X Y g P f f0 g0 y c) = Cyl_rect X Y g P f f0 g0 y c').
+
 
 Inductive isInhab (X:Type) : Type :=
     | proj : X -> isInhab X
@@ -168,6 +235,13 @@ isInhab_rect
        (forall (y : isInhab X) (h : P y) (y' : isInhab X) (h0 : P y'),
         transp P (contr X y y') h = h0) -> forall i : isInhab X, P i
 *)
+Check (isInhab_rect2 :
+       forall (X : Type) (P : isInhab X -> Type)
+       (f:forall x : X, P (proj X x))
+       (g:forall (y : isInhab X) (h : P y) (y' : isInhab X) (h0 : P y'),
+        transp P (contr X y y') h = h0)
+       (i i': isInhab X) (e:i=i'),
+       transp P e (isInhab_rect X P f g i) = isInhab_rect X P f g i').
 
 (* Recursive 1-constructors not allowed yet (+ defines 2-constructor):
 Inductive tr0 (X:Type) : Type :=
@@ -199,7 +273,7 @@ with paths :=
 | relate (x y : A) (h:R x y) : (qproj x) = (qproj y)
 | contr1 (x y : quotient A R) (p q : x=y) : p = q.
  *)
-
+Check τ_0_rect2.
 
 
 Inductive hpushout {A B C : Type} (f : A -> B) (g : A -> C) : Type :=
@@ -216,3 +290,4 @@ hpushout_rect
        (forall a : A, transp P (glue A B C f g a) (f0 (f a)) = f1 (g a)) ->
        forall h : hpushout f g, P h
 *)
+Check hpushout_rect2.
